Leanduction/SparseRecursor.lean
@@ -6,24 +6,25 @@ open Lean Elab Meta
 
 namespace SparseRecursor
 
-partial def replaceNestedMotives (indVals : List InductiveVal) (realMotives : Array Expr) (nestedMotives : Array Expr) : MetaM (Array Expr) := do
-  go 0 #[]
+partial def replaceNestedMotivesAndMinors (indVals : List InductiveVal) (realMotives : Array Expr) (nestedMotives : Array Expr) : MetaM (Array Expr × Array Expr) := do
+  go 0 #[] #[]
 where
-  go (i : Nat) (acc : Array Expr) : MetaM (Array Expr) :=
+  go (i : Nat) (motivesReplacements minorsReplacements : Array Expr): MetaM (Array Expr × Array Expr) :=
     if _ : i < nestedMotives.size then do
       -- Ds -> Is As Ds -> Prop
-      let nestedMotive : Expr ← forallTelescope (← inferType nestedMotives[i]) fun xs ty => do
+      let nestedMotiveAndMinors : (Expr × Array Expr) ← forallTelescope (← inferType nestedMotives[i]) fun xs ty => do
         let major := xs[xs.size-1]!
         let majorType ← inferType major
-        let ty ← nestedMotive majorType
+        let (ty,minors) ← nestedMotiveAndMinors majorType false
         let ty := mkApp ty major
-        mkLambdaFVars xs ty
-      logInfo m!"nestedMotive : {nestedMotive}"
-      go (i+1) (acc.push nestedMotive)
+        let ty ← mkLambdaFVars xs ty
+        return (ty,minors)
+      logInfo m!"nestedMotive : {nestedMotiveAndMinors}"
+      go (i+1) (motivesReplacements.push nestedMotiveAndMinors.1) (minorsReplacements.append nestedMotiveAndMinors.2)
     else
-      return acc
+      return (motivesReplacements,minorsReplacements)
 
-  nestedMotive (motiveType : Expr) : MetaM Expr := do
+  nestedMotiveAndMinors (motiveType : Expr) (noMinors : Bool) : MetaM (if noMinors then Expr else Expr × Array Expr) := do
     logInfo m!"nestedMotive {motiveType}"
     motiveType.withApp fun fn args =>  do
       let nestedIndName := fn.constName!
@@ -32,16 +33,16 @@ where
       let nestedParamsMask ← NestedPositivity.positiveParams nestedIndVal
       let sparseNestedIndName := SparseParametricityTranslation.sparseName fn.constName!
       let ty := mkAppN (mkConst sparseNestedIndName fn.constLevels!) nestedParams
-      logInfo m!"step 1 : {ty}"
-      let preds ← nestedParams.mapIdxM fun idx e => if nestedParamsMask[idx]! then return some ( ← genPred e) else pure none
-      logInfo m!"preds : {preds}"
+      let preds ← nestedParams.mapIdxM fun idx e => if nestedParamsMask[idx]! then return some (← genPred e) else pure none
       let ty := mkAppN ty (preds.filterMap id)
-      logInfo m!"step 2 : {ty}"
       let ty := mkAppN ty args[nestedIndVal.numParams...*]
-      logInfo m!"step 3 : {ty}"
-      logInfo m!"step 4 : {ty}"
-      logInfo m!"step 5 : {ty}"
-      return ty
+      match noMinors with
+        | true => return ty
+        | false => do
+          let sparseNestedIndVal ← getConstInfoInduct sparseNestedIndName
+          let minors := sparseNestedIndVal.ctors.toArray.map fun ctorName =>
+              mkAppN (mkAppN (mkConst ctorName fn.constLevels!) nestedParams) (preds.filterMap id)
+          return (ty,minors)
 
   genPred (param : Expr) : MetaM Expr := do
     logInfo m!"genPred {param}"
@@ -53,26 +54,25 @@ where
         let fnName := fn.constName!
         if let some indIdx := indVals[0]!.all.findIdx? (· == fnName) then
           let ty := realMotives[indIdx]!
-          let ty := mkAppN ty args[indVals[indIdx]!.numIndices...*]
-          let ty := ty
+          let ty := mkAppN ty args[indVals[indIdx]!.numParams...*]
           withLocalDeclD `f param fun f => do
             let ty := mkApp ty (mkAppN f xs)
             let ty ← mkForallFVars xs ty
             let motive ← mkLambdaFVars #[f] ty
             return motive
         else
-          let ty ← nestedMotive ty
+          let ty ← nestedMotiveAndMinors ty true
           withLocalDeclD `f param fun f => do
             let ty := mkApp ty (mkAppN f xs)
             let ty ← mkForallFVars xs ty
             let motive ← mkLambdaFVars #[f] ty
             return motive
 
--- TODO generate the term at the same time ?
-def type (indName : Name) : MetaM Expr := do
+def genSparseRec (indName : Name) : TermElabM Unit := do
   let info ← getConstInfoInduct indName
   let indVals ← info.all.mapM getConstInfoInduct
-  let recInfo ← getConstInfoRec (info.name ++ `rec)
+  let recName := info.name ++ `rec
+  let recInfo ← getConstInfoRec recName
   let recTypeToProp := match recInfo.levelParams with
     | [] => recInfo.type
     | motiveUniv::_ => recInfo.type.instantiateLevelParams [motiveUniv] [0]
@@ -81,7 +81,7 @@ def type (indName : Name) : MetaM Expr := do
     let indices_and_major := xs[recInfo.getFirstIndexIdx...*]
     let motives := xs[info.numParams...info.numParams + info.all.length]
     let nestedMotives := xs[(info.numParams + info.all.length)...recInfo.getFirstMinorIdx]
-    let sparseForNestedMotives ←  replaceNestedMotives indVals motives nestedMotives
+    let (sparseForNestedMotives,nestedsMinors) ← replaceNestedMotivesAndMinors indVals motives nestedMotives
     logInfo m!"sparseForNestedMotives : {sparseForNestedMotives}"
     let numMinors := indVals.foldl (init := 0) (fun acc ind => acc + ind.ctors.length)
     let oldMinors := xs[recInfo.getFirstMinorIdx...recInfo.getFirstMinorIdx + numMinors]
@@ -94,6 +94,27 @@ def type (indName : Name) : MetaM Expr := do
       let ty ← mkForallFVars motives ty
       let ty ← mkForallFVars params ty
       Meta.check ty
-      return ty
-
+      let recUnivs := match recInfo.levelParams with
+        | [] => []
+        | _::us => 0::us.map Level.param
+      let te := mkConst recName recUnivs
+      let te := mkAppN te params
+      let te := mkAppN te motives
+      let te := mkAppN te sparseForNestedMotives
+      let te := mkAppN te minors
+      let te := mkAppN te nestedsMinors
+      let te ← mkLambdaFVars minors te
+      let te ← mkLambdaFVars motives te
+      let te ← mkLambdaFVars params te
+      logInfo m!"term : {te}"
+      Meta.check te
+      addDecl <| .defnDecl {
+        name := indName ++ `rec_sparse
+        levelParams := match recInfo.levelParams with | [] => [] | _::tl => tl
+        type := ty
+        value := te
+        hints := .regular 0 --TODO figure out how important that is ?
+        safety := .safe
+        }
+      Term.applyAttributes (indName ++ `rec_sparse) #[{name := `induction_eliminator}]
 end SparseRecursor
